base <https://pod.inrupt.com/>
# BaseIRI determines if this document is Server-wide description,
# or only applies to a specific Pod.
#base <https://pod.inrupt.com/{username}/>

prefix rdf: <http://www.w3.org/1999/02/22-rdf-syntax-ns#>
prefix rdfs: <http://www.w3.org/2000/01/rdf-schema#>
prefix xsd: <http://www.w3.org/2001/XMLSchema#>
prefix owl: <http://www.w3.org/2002/07/owl#>
prefix dcterms: <http://purl.org/dc/terms/>
prefix skos-xl: <http://www.w3.org/2008/05/skos-xl#>
prefix ldp: <http://www.w3.org/ns/ldp#>
prefix as: <https://www.w3.org/ns/activitystreams#>
prefix sparql-sd: <http://www.w3.org/ns/sparql-service-description#>
prefix hydra: <http://www.w3.org/ns/hydra/core#>
prefix vann: <http://purl.org/vocab/vann/>
prefix schema: <http://schema.org/>
prefix solid: <http://www.w3.org/ns/solid/terms#>

#
# We could also put all these terms directly into the existing
# Solid Terms vocabulary, but perhaps good to keep separate
# during discussions…
#
prefix solid-sd: <http://www.w3.org/ns/solid/service-description#>

solid-sd:
   a owl:Ontology;
   owl:versionInfo "0.1" ;
   dcterms:title "Solid Service Description vocabulary"@en ;
   dcterms:description """The Solid Service Description vocabulary
describes the services provided by a Solid Server."""@en ;
   dcterms:creator <https://inrupt.com/profile/card/#us> ;
   dcterms:issued "2019/11/08"^^xsd:date ;
   dcterms:license "http://purl.org/NET/rdflicense/MIT1.0.ttl" ;
   vann:preferredNamespacePrefix "solid-sd" ;
   vann:preferredNamespaceUri "http://www.w3.org/ns/solid/service-description#" .

solid-sd:Service a rdfs:Class ;
   rdfs:label "Solid Service"@en ;
   rdfs:comment """A Solid Service is some function provided by a Solid Server,
e.g., to search a Pod, send a notification to an Inbox, logout of a Pod,
etc."""@en .

solid-sd:Feature a rdfs:Class ;
    rdfs:label "Feature" ;
    rdfs:comment """An instance of solid-sd:Feature represents a feature of a
 Solid service. Specific types of features might include protocols (or
 sub-protocols)"""@en .

solid-sd:Protocol a rdfs:Class ;
    rdfs:subClassOf solid-sd:Feature ;
    rdfs:label "Protocol" ;
    rdfs:comment """An instance of solid-sd:Protocol represents one specific
 protocol (or sub-protocol)."""@en .


solid-sd:endpoint a rdf:Property ;
   rdfs:label "Solid Endpoint"@en ;
   rdfs:comment """A Solid Endpoint is the URL through which an agent requests
that a Solid Service performs its function, e.g., the SPARQL endpoint for a
"Search my Pod Solid Service."""@en .


solid-sd:feature a rdf:Property ;
           rdfs:domain solid-sd:Service ;
           rdfs:range solid-sd:Feature ;
           rdfs:label "feature" ;
           rdfs:comment """Relates an instance of solid-sd:Service with a
 resource representing a supported feature."""@en .

solid-sd:supportedProtocol a rdf:Property ;
    rdfs:subPropertyOf solid-sd:feature ;
    rdfs:label "supported language"@en ;
    rdfs:comment """Relates an instance of solid-sd:Service to a protocol (or
 sub-protocol) that it implements (e.g., a WebSocket service might implement
 multiple, or just one, sub-protocols."""@en ;
    schema:domainIncludes solid-sd:Service ;
    schema:rangeIncludes solid-sd:Protocol .


#
# Pre-defined Solid Services...
#
# These services also act as pre-defined extension Link relation IRIs...
#
# For convenience and/or to promote reuse (i.e., to support interoperability,
# whereby multiple parties agree on the semantics of relationships between
# resources), Link relations are expected to be registered with IANA:
#   https://www.iana.org/assignments/link-relations/link-relations.xhtml
#
# Note: The question of "link relations for RDF" goes back to at least 2013:
#   https://github.com/mnot/I-D/issues/39
#
# There are two kinds of link relation types: registered and extension.
# Registered types are short descriptive strings (e.g., 'about', 'first',
# 'previous'), whereas extension types are URIs. Due to the web native nature of
# Solid, we use extension types.
#
# Section 2.1.2 (https://httpwg.org/specs/rfc8288.html#rfc.section.2.1.2) of the
# RFC states that: "Because of this, all-lowercase URIs SHOULD be used for
# extension relations", however by way of example, the W3C Time ontology
# explicitly uses mixed case link relations: https://www.w3.org/TR/owl-time/#iana-links
# and our currently favored guidance on RDF terms is to use mixed-case too.
#
# We use the Activity Streams vocabulary for describing our extension Link
# relations, specifically 'as:rel'.
#
# A machine-readable Solid service description document can be advertised on a
# per-resource basis using the existing IANA registered 'service-desc'.
# Should this describe the services provided by the Solid server as a whole, or
# to the services available/visible only in the context of the request resource?
# I.e., only available for the currently logged-in user (e.g., if I were an
# anonymous user requesting a public document in Alice's Pod, would I expect to
# have visibility into Alice's PodSwitch service (although I could probably
# still discover it via a template URI in the Server-wide description
# document)?
#
# GET http://pod.com/alice/private/photo/family
#   Link: <http://pod.com/.well-known/solid> rel="service-desc"
#   Link: <http://pod.com/alice/service-qpf> rel="http://www.w3.org/ns/solid/service-description#serviceQpf"
#   Link: <http://pod.com/powerswitch/alice> rel="http://www.w3.org/ns/solid/service-description#servicePowerSwitch"


solid-sd:serviceSparql a rdf:Property, as:rel ;
   rdfs:label "Solid Service Sparql"@en ;
   rdfs:comment """A Solid Service providing SPARQL query capability - could be
 across data within a single Pod, or across all Pods hosted by a Solid Server
 provider."""@en .

solid-sd:serviceGraphql a rdf:Property, as:rel ;
   rdfs:label "Solid Service GraphQL"@en ;
   rdfs:comment """A Solid Service providing GraphQL query capability. This
 service initially provides authenticated and authorized access to sensitive
 access control data associated with resources in Pods."""@en .

solid-sd:servicePowerSwitch a rdf:Property, as:rel ;
   rdfs:label "Solid Service Power Switch"@en ;
   rdfs:comment """A Solid Service providing the ability to 'power off' a Pod.
 This is useful in cases where a Pod owner wishes to completely disable all
 access to their entire Pod (e.g., in the case that they suspect access has been
 compromised)."""@en .

solid-sd:servicePodRegistration a rdf:Property, as:rel ;
    rdfs:label "Solid Service Pod Registration"@en ;
    rdfs:comment """A Solid Service providing the ability to register a new
 a Pod. Generally we’d expect this service to be provided by a Solid
 Identity Provider, although some server implementations may wish to offer this service directly themselves too."""@en .

solid-sd:serviceWebSocket a rdf:Property, as:rel ;
    rdfs:label "Solid Service WebSocket"@en ;
    rdfs:comment """A Solid Service providing the ability to subscribe to
 resource change events via a WebSocket connection."""@en .

#
# WebSocket sub-protocols.
# Note: these values cannot be IRIs (see the associated rdfs:seeAlso links),
# so we use skos-xl Labels to provide the literal forms to actually use as the
# value of HTTP request 'Sec-WebSocket-Protocol' headers.
#
solid-sd:WebSocketSubProtocol0.1 a solid-sd:Protocol ;
    skos-xl:prefLabel solid-sd:WebSocketSubProtocol0.2Label ;
    rdfs:seeAlso <https://github.com/solid/solid-spec/blob/master/api-websockets.md> ,
                 <https://developer.mozilla.org/en-US/docs/Web/API/WebSockets_API/Writing_WebSocket_servers#subprotocols> ,
                 <https://tools.ietf.org/html/rfc6455#section-4.1> ,
                 <https://bugs.chromium.org/p/chromium/issues/detail?id=398407> ,
                 solid-sd:WebSocketSubProtocol0.1Label ;
    rdfs:label "WebSocket sub-protocol 0.1 (legacy)"@en ;
    rdfs:comment """A solid-sd:Protocol representing the original Solid
 WebSocket protocol.
 Note: the value of this protocol cannot be an IRI (see the rdfs:seeAlso links),
 which is why we must use a label instead."""@en .

solid-sd:WebSocketSubProtocol0.1Label a skos-xl:Label ;
    rdfs:seeAlso solid-sd:WebSocketSubProtocol0.1 ;
    skos-xl:literalForm "solid-0.1" .

solid-sd:WebSocketSubProtocol0.2 a solid-sd:Protocol ;
    skos-xl:prefLabel solid-sd:WebSocketSubProtocol0.2Label ;
    rdfs:seeAlso <https://developer.mozilla.org/en-US/docs/Web/API/WebSockets_API/Writing_WebSocket_servers#subprotocols> ,
                 <https://tools.ietf.org/html/rfc6455#section-4.1> ,
                 <https://bugs.chromium.org/p/chromium/issues/detail?id=398407> ,
                 solid-sd:WebSocketSubProtocol0.2Label ;
    rdfs:label "WebSocket sub-protocol v0.2"@en ;
    rdfs:comment """A solid-sd:Protocol representing version 0.2 of the Solid
 WebSocket sub-protocol. This version supports event payloads using RDF (e.g.,
 serialized as JSON-LD) to support rich, interoperable and extensible event
 meta-data.
 Note: the value of this protocol cannot be an IRI (see the rdfs:seeAlso links),
 which is why we must use a label instead."""@en .

solid-sd:WebSocketSubProtocol0.2Label a skos-xl:Label ;
    rdfs:seeAlso solid-sd:WebSocketSubProtocol0.2 ;
    skos-xl:literalForm "solid-0.2" .

#################################################################
#
# Instance data for an actual Solid Server Description document.
#
#################################################################

</.well-known/solid>
   solid-sd:serviceSparql <service-sparql> ;
   solid-sd:serviceGraphql <service-graphql> ;
   solid-sd:serviceQpf <service-qpf> ;
   solid-sd:servicePowerSwitch <service-power-switch> ;
   solid-sd:servicePodRegistration <service-pod-registration> .

   #
   # THESE GUYS ARE NOT MODELLED YET…
   #
#   solid-sd:notificationGatewayEndpoint <{NOTIFICATION_GATEWAY_URL}> ;
#   solid:loginEndpoint <{LOGIN_URL}> ;
#   solid:logoutEndpoint <{LOGOUT_URL}> .

   # These predicates might only apply to Pod-specific Service Descriptions.
   # solid:podOwner <{WEBID}> ;
   # ldp:inbox <{INBOX_URL}> ;

<service-sparql> a sparql-sd:Service ;
   rdfs:comment """Just for illustration, here we use the existing SPARQL
 Service Description vocabulary to describe a hypothetical SPARQL endpoint."""@en ;
   sparql-sd:endpoint <sparql> ;
   sparql-sd:supportedLanguage sparql-sd:SPARQL11Query, sparql-sd:SPARQL11Update ;
   sparql-sd:extensionFunction solid-sd:AcpResourceByAgent .

<service-graphql> a solid-sd:Service ;
   solid-sd:endpoint <query-graphql> ;
   dcterms:created "2021-02-01"^^xsd:date .

<service-qpf> a solid-sd:Service ;
   solid-sd:endpoint <query-qpf> ;
   hydra:template "{?endpoint}{?s,p,o,g}" ;
   hydra:search [
       hydra:mapping [
           hydra:property rdf:subject ;
           hydra:variable "s"
       ], [
           hydra:property rdf:predicate ;
           hydra:variable "p"
       ], [
           hydra:property rdf:object ;
           hydra:variable "o"
       ], [
           hydra:property sparql-sd:graph ;
           hydra:variable "g"
       ]
   ] .

<service-power-switch> a solid-sd:Service ;
   solid-sd:endpoint <power-switch> ;
   dcterms:created "2021-02-01"^^xsd:date ;
   hydra:template "{?pod}/powerSwitch" ;
   hydra:search [
       hydra:mapping [
           hydra:property solid:podRoot ;
           hydra:variable "pod"
       ]
   ] .

<service-pod-registration> a solid-sd:Service ;
   solid-sd:endpoint <pod-registration> ;
   dcterms:created "2021-02-01"^^xsd:date ;
   hydra:template "{?endpoint}{?username,password}" ;
   hydra:search [
       hydra:mapping [
           hydra:property solid:username ;
           hydra:variable "username"
       ] ,
       hydra:mapping [
           hydra:property solid:password ;
           hydra:variable "password"
       ]
   ] .

<service-web-socket> a solid-sd:Service ;
   solid-sd:endpoint <pod-registration> ;
   dcterms:created "2021-02-01"^^xsd:date .
