prefix rdf:      <http://www.w3.org/1999/02/22-rdf-syntax-ns#>
prefix rdfs:     <http://www.w3.org/2000/01/rdf-schema#>
prefix xsd:      <http://www.w3.org/2001/XMLSchema#>
prefix owl:      <http://www.w3.org/2002/07/owl#>
prefix vann:     <http://purl.org/vocab/vann/>
prefix dcterms:  <http://purl.org/dc/terms/>
prefix skos:     <http://www.w3.org/2004/02/skos/core#>
prefix skosxl:   <http://www.w3.org/2008/05/skos-xl#>
prefix cc:       <http://creativecommons.org/ns#>
prefix schema:   <http://schema.org/>

prefix inrupt_gen:    <https://inrupt.com/vocab/tool/artifact_generator#>
prefix inrupt_common: <https://inrupt.com/vocab/common#>

#
# Describe our vocabulary - i.e., an English description, its version, who created it, its
# suggested prefix, its license, etc.
#
inrupt_common: a owl:Ontology, inrupt_gen:Ontology ;
	owl:versionInfo "0.0.1" ;
	owl:versionIRI <https://inrupt.com/vocab/common/0.0.1> ;
    dcterms:title "Inrupt common vocabulary"@en ;
    dcterms:title "Inrupt vocabulario común"@es ;
	dcterms:description "The Inrupt common vocabulary - just commonly used terms across all Inrupt products and services."@en ;
	dcterms:description "El Inrupt vocabulario común: términos de uso común en todos los productos y servicios de Inrupt."@es ;
	dcterms:creator <https://inrupt.com/profile/card/#us> ;
	dcterms:issued "2019/11/08"^^xsd:date ;
	dcterms:license "http://purl.org/NET/rdflicense/MIT1.0.ttl" ;
	vann:preferredNamespacePrefix "inrupt_common" ;
	vann:preferredNamespaceUri "https://inrupt.com/vocab/common#" .

#
# Acronym support.
#
inrupt_common:Acronym a rdfs:Class ;
    rdfs:isDefinedBy inrupt_common: ;
    rdfs:label "Acronym"@en ;
    rdfs:label "Acrónimo"@es ;
    rdfs:comment """The class of all acronyms."""@en ;
    rdfs:comment """La clase de todas las siglas."""@es .

inrupt_common:acronym rdfs:subPropertyOf skosxl:labelRelation ;
    rdfs:isDefinedBy inrupt_common: ;
    rdfs:label "Acronym"@en ;
    rdfs:label "Acrónimo"@es ;
    rdfs:comment """An instance of an acronym - expected to be used on terminology, phrases, or concepts."""@en ;
    rdfs:comment """Una instancia de un acrónimo: se espera que se use en terminología, frases o conceptos."""@es ;
    schema:domainIncludes skosxl:Label ;
    schema:rangeIncludes skosxl:Label .

inrupt_common:acronymExpandedForm a rdfs:Property ;
    rdfs:isDefinedBy inrupt_common: ;
    rdfs:label "Acronym expanded form"@en ;
    rdfs:label "Forma expandida de siglas"@es ;
    rdfs:comment """An expanded form for an acronym, expected to provide more detail on what an acronym actually refers to."""@en ;
    rdfs:comment """Una forma ampliada de un acrónimo, que se espera que proporcione más detalles sobre a qué se refiere realmente un acrónimo."""@es ;
    schema:domainIncludes skosxl:Label ;
    schema:rangeIncludes skosxl:Label .


#
# Common error messages.
#
inrupt_common:errFailedToProcessIncomingRdf a skosxl:Label ;
	skos:definition "Failed to process incoming message as RDF."@en ;
    skos:definition "No se pudo procesar el mensaje entrante como RDF."@es .

inrupt_common:msgRequestValidatedAsRdf a skosxl:Label ;
    skos:definition "Incoming request validated as RDF (it has [{{0}}] triples!)."@en ;
	skos:definition "Solicitud entrante validada como RDF (¡tiene [{{0}}] triples!)."@es .


#
# Customer identifiers.
#
inrupt_common:CustomerId a rdfs:Class ;
    rdfs:isDefinedBy inrupt_common: ;
    rdfs:label "Class of customer identifiers"@en ;
    rdfs:label "Clase de identificadores de clientes"@es ;
    rdfs:comment """The class of customer identifiers (e.g., identifiers for customers from legacy
 systems, or 3rd-party systems, or separate internal systems, etc.)."""@en ;
    rdfs:comment """La clase de identificadores de clientes (p. Ej., Identificadores de clientes de
 legacy sistemas o sistemas de terceros, o sistemas internos separados, etc.)."""@es .


inrupt_common:customerId a rdf:Property ;
    rdfs:isDefinedBy inrupt_common: ;
    rdfs:label "Customer identifier"@en ;
    rdfs:label "Identificador de cliente"@es ;
    rdfs:comment """A generic customer identifier (e.g., an identifier for a customer from a legacy
 system, or a 3rd-party system, or a separate internal system, etc.)."""@en ;
    rdfs:comment """Un identificador de cliente genérico (por ejemplo, un identificador de un
 cliente de un sistema heredado, un sistema de terceros o un sistema interno separado, etc.)."""@es .

#
# Authentication.
#
inrupt_common:AuthenticationResponse a rdfs:Class ;
    rdfs:isDefinedBy inrupt_common: ;
    rdfs:label "Class of Authentication Responses"@en ;
    rdfs:label "Clase de respuestas de autenticación"@es ;
    rdfs:comment """Type used to denote a response from an authentication request (expected to
 contain things like access tokens, user IDs, account IDs, etc., when authenticating with an API)."""@en ;
    rdfs:comment """Tipo utilizado para denotar una respuesta de una solicitud de autenticación (se
 espera que contenga elementos como tokens de acceso, ID de usuario, ID de cuenta, etc., al
 autenticarse con una API)."""@es .


inrupt_common:authenticationTokenAsJwt a rdf:Property ;
    rdfs:isDefinedBy inrupt_common: ;
    rdfs:label "Authentication token as JWT"@en ;
    rdfs:label "Token de autenticación como JWT"@es ;
    rdfs:comment """An authentication token encoded as a JSON Web Token (JWT). This JWT may
 contain not just an access code, but also user account IDs or other information."""@en ;
    rdfs:comment """Un token de autenticación codificado como JSON Web Token (JWT). Este JWT puede
 contener no solo un código de acceso, sino también ID de cuenta de usuario u otra información."""@es .

inrupt_common:accessTokenAsString a rdf:Property ;
    rdfs:isDefinedBy inrupt_common: ;
    rdfs:label "Access token (as string)"@en ;
    rdfs:label "Token de acceso (como cadena)"@es ;
    rdfs:comment """An access token, typically used to access an API, represented as a simple string value."""@en ;
    rdfs:comment """Un token de acceso, normalmente utilizado para acceder a una API, representado
 como un valor de cadena simple."""@es .
