prefix rdf:      <http://www.w3.org/1999/02/22-rdf-syntax-ns#>
prefix rdfs:     <http://www.w3.org/2000/01/rdf-schema#>
prefix xsd:      <http://www.w3.org/2001/XMLSchema#>
prefix owl:      <http://www.w3.org/2002/07/owl#>
prefix skos:     <http://www.w3.org/2004/02/skos/core#>
prefix sh:       <http://www.w3.org/ns/shacl#>
prefix dcterms:  <http://purl.org/dc/terms/>
prefix dalicc:   <http://dalicc.net/licenselibrary/>

prefix inrupt_gen: <https://w3id.org/inrupt/namespace/vocab/tool/artifact_generator/>
prefix inrupt_fair: <https://w3id.org/inrupt/vocab/tool/bestPractice/fair/>

#
# Describe our vocabulary - i.e., an English description, its version, who
# created it, its suggested prefix, its license, etc.
#
inrupt_fair:_Ontology a owl:Ontology , inrupt_gen:Ontology ;
	owl:versionInfo "0.0.1" ;
    owl:versionIRI <https://w3id.org/inrupt/vocab/tool/bestPractice/fair/0.0.1> ;
 	dcterms:title "FAIR principles"@en ;
	dcterms:description "The FAIR principles, as published by Scientific Data in 2016."@en ;
	rdfs:seeAlso "https://www.go-fair.org/fair-principles/"^^xsd:anyURI ;
	rdfs:seeAlso "https://www.go-fair.org/go-fair-initiative/"^^xsd:anyURI ;
	dcterms:creator <https://w3id.com/inrupt/namespace/webid/inrupt> ;
	dcterms:issued "2022/12/05"^^xsd:date ;
	dcterms:license dalicc:MIT ;
    sh:declare inrupt_fair:_PrefixDeclaration .

inrupt_fair:_PrefixDeclaration a sh:PrefixDeclaration ;
    sh:prefix "inrupt_fair" ;
    sh:namespace "https://w3id.org/inrupt/vocab/tool/bestPractice/fair/" .

#
# Terms...
#
inrupt_fair:Findable a rdfs:Class, skos:Concept ;
    rdfs:isDefinedBy inrupt_fair:_Ontology ;
    rdfs:label "Findable"@en ;
    rdfs:comment """Make the ontology findable on the Web."""@en .

inrupt_fair:_F1_globallyUniquePersistentIdentifier a owl:NamedIndividual, skos:Concept ;
    rdfs:isDefinedBy inrupt_fair:_Ontology ;
    rdfs:label "Globally unique and persistent identifier"@en ;
    rdfs:comment """F1. (meta)data are assigned a globally unique and persistent identifier."""@en ;
    skos:broader inrupt_fair:Findable .

inrupt_fair:_F2_richMetadata a owl:NamedIndividual, skos:Concept ;
    rdfs:isDefinedBy inrupt_fair:_Ontology ;
    rdfs:label "Rich metadata"@en ;
    rdfs:comment """F2. data are described with rich metadata (defined by R1 'inrupt_fair:_R1_richAttributes')."""@en ;
    rdfs:seeAlso inrupt_fair:_R1_richAttributes ;
    skos:broader inrupt_fair:Findable .



inrupt_fair:Reusable a rdfs:Class, skos:Concept ;
    rdfs:isDefinedBy inrupt_fair:_Ontology ;
    rdfs:label "Reusable"@en ;
    rdfs:comment """To be Reusable."""@en .

inrupt_fair:_R1_richAttributes a owl:NamedIndividual, skos:Concept ;
    rdfs:isDefinedBy inrupt_fair:_Ontology ;
    rdfs:label "Rich attributes"@en ;
    rdfs:comment """R1. meta(data) are richly described with a plurality of accurate and relevant attributes."""@en ;
    rdfs:seeAlso inrupt_fair:_F2_richMetadata ;
    skos:broader inrupt_fair:Reusable .
