prefix rdf:      <http://www.w3.org/1999/02/22-rdf-syntax-ns#>
prefix rdfs:     <http://www.w3.org/2000/01/rdf-schema#>
prefix xsd:      <http://www.w3.org/2001/XMLSchema#>
prefix owl:      <http://www.w3.org/2002/07/owl#>
prefix sh:       <http://www.w3.org/ns/shacl#>
prefix dcterms:  <http://purl.org/dc/terms/>
prefix skos:     <http://www.w3.org/2004/02/skos/core#>
prefix skosxl:   <http://www.w3.org/2008/05/skos-xl#>
prefix cc:       <http://creativecommons.org/ns#>
prefix schema:   <https://schema.org/>
prefix dalicc:   <http://dalicc.net/licenselibrary/>

# This vocab is 'old', and contains no owl:NamedIndividual's for the various
# states a term can be in (such as 'standard', 'deprecated', 'experimental',
# etc.), but it is W3C-hosted!
# Suggests the need for the creation of a more 'modern' vocab perhaps...
prefix vs:       <http://www.w3.org/2003/06/sw-vocab-status/ns#>

prefix inrupt_gen:    <https://w3id.org/inrupt/namespace/vocab/tool/artifact_generator/>
prefix inrupt_common: <https://w3id.org/inrupt/namespace/vocab/common/>

#
# Describe our vocabulary - i.e., an English description, its version, who created it, its
# suggested prefix, its license, etc.
#
inrupt_common: a owl:Ontology , inrupt_gen:Ontology ;
    owl:versionInfo "0.0.1" ;
    owl:versionIRI <https://w3id.org/inrupt/namespace/vocab/common/0.0.1> ;
    dcterms:title "Inrupt common vocabulary"@en ;
    dcterms:title "Inrupt vocabulario común"@es ;
    dcterms:description "The Inrupt common vocabulary - just commonly used terms across all Inrupt products and services."@en ;
    dcterms:description "El Inrupt vocabulario común: términos de uso común en todos los productos y servicios de Inrupt."@es ;
    dcterms:creator <https://w3id.com/inrupt/namespace/webid/inrupt> ;
    dcterms:issued "2019/11/08"^^xsd:date ;
    dcterms:license dalicc:MIT ;
    sh:declare inrupt_common:_PrefixDeclaration .

inrupt_common:_PrefixDeclaration a sh:PrefixDeclaration ;
    sh:prefix "inrupt_common" ;
    sh:namespace "https://w3id.org/inrupt/namespace/vocab/common/"^^xsd:anyURI .

#
# We did have terms to represent the very generic concept of a 'device'
# (e.g., could be a mobile phone, or a home appliance, or any Internet of
# Things (IoT) device, etc.), but we removed them in favor of reusing
# existing vocabs such as SOSA (http://www.w3.org/ns/sosa), SSN
# (http://www.w3.org/ns/ssn), or SAREF.
#
# Note: Schema.org has a 'device' term, but apparently it's been superceded by
# 'https://schema.org/availableOnDevice' (according to
# 'https://schema.org/SoftwareApplication').
#

#
# Acronym support.
#
inrupt_common:Acronym a rdfs:Class ;
    rdfs:isDefinedBy inrupt_common: ;
    rdfs:label "Acronym"@en ;
    rdfs:label "Acrónimo"@es ;
    rdfs:comment """The class of all acronyms."""@en ;
    rdfs:comment """La clase de todas las siglas."""@es .

inrupt_common:acronym rdfs:subPropertyOf skosxl:labelRelation ;
    rdfs:isDefinedBy inrupt_common: ;
    rdfs:label "Acronym"@en ;
    rdfs:label "Acrónimo"@es ;
    rdfs:comment """An instance of an acronym - expected to be used on terminology, phrases, or concepts."""@en ;
    rdfs:comment """Una instancia de un acrónimo: se espera que se use en terminología, frases o conceptos."""@es ;
    schema:domainIncludes skosxl:Label ;
    schema:rangeIncludes skosxl:Label .

inrupt_common:acronymExpandedForm a rdfs:Property ;
    rdfs:isDefinedBy inrupt_common: ;
    rdfs:label "Acronym expanded form"@en ;
    rdfs:label "Forma expandida de siglas"@es ;
    rdfs:comment """An expanded form for an acronym, expected to provide more detail on what an acronym actually refers to."""@en ;
    rdfs:comment """Una forma ampliada de un acrónimo, que se espera que proporcione más detalles sobre a qué se refiere realmente un acrónimo."""@es ;
    schema:domainIncludes skosxl:Label ;
    schema:rangeIncludes skosxl:Label .


#
# Common error messages.
#
inrupt_common:errFailedToProcessIncomingRdf a rdfs:Literal ;
    skos:definition "Failed to process incoming message as RDF."@en ;
    skos:definition "No se pudo procesar el mensaje entrante como RDF."@es .

inrupt_common:msgRequestValidatedAsRdf a rdfs:Literal ;
    skos:definition "Incoming request validated as RDF (it has [{{0}}] triples!)."@en ;
    skos:definition "Solicitud entrante validada como RDF (¡tiene [{{0}}] triples!)."@es .


#
# Customer identifiers.
#
inrupt_common:CustomerId a rdfs:Class ;
    rdfs:isDefinedBy inrupt_common: ;
    rdfs:label "Class of customer identifiers"@en ;
    rdfs:label "Clase de identificadores de clientes"@es ;
    rdfs:comment """The class of customer identifiers (e.g., identifiers for customers from legacy
 systems, or 3rd-party systems, or separate internal systems, etc.)."""@en ;
    rdfs:comment """La clase de identificadores de clientes (p. Ej., Identificadores de clientes de
 legacy sistemas o sistemas de terceros, o sistemas internos separados, etc.)."""@es .


inrupt_common:partialIdHint a rdf:Property ;
    rdfs:isDefinedBy inrupt_common: ;
    rdfs:label "Partial ID hint"@en ;
    rdfs:label "Sugerencia de ID parcial"@es ;
    rdfs:comment """A partial identifier (useful as a 'hint'), but not a full
 IRI. This ID can be useful as a form of helpful 'correlation ID' - for
 instance, when a complex process has many constituent resources (e.g., an
 overall questionnaire process may aggregate resources for participant
 invitation; the questions being asked; the answers given; the sharing of
 those answers; the anonymization of those answers; the aggregation of those
 answers into an overall dataset; the geneation of an analysis report; etc.).
  For helpful tracking of all these resources, we may choose to use a
 consistent ID as part of the IRI of each constituent resource, but where each
 resource is hosted in a Pod related to that process stakeholder, and
 therefore the IRI for each resource (that is effectively 'aggregated'
 together to form the entire overall process) can be completely independent
 and different - so it's really important to remember that the use of this ID
 should always be purely optional (as the IRIs themselves should always be
 considered as being completely opaque, and should never encode  meaningful
 semantics in the 'parts' of their IRIs!)."""@en ;
    rdfs:comment """Un identificador parcial (útil como 'pista'), pero no un identificador completo
 IRI. Esta identificación puede ser útil como una forma de 'identificación de correlación' útil, por
 ejemplo, cuando un proceso complejo tiene muchos recursos constituyentes (por ejemplo, un
 el proceso general del cuestionario puede agregar recursos para los participantes
 invitación; las preguntas que se hacen; las respuestas dadas; el compartir de
 esas respuestas; la anonimización de esas respuestas; la suma de esos
 respuestas en un conjunto de datos general; la generación de un informe de análisis; etc.).
  Para un seguimiento útil de todos estos recursos, podemos optar por utilizar un
 ID consistente como parte del IRI de cada recurso constituyente, pero donde cada
 el recurso está alojado en un Pod relacionado con esa parte interesada del proceso, y
 por lo tanto, el IRI para cada recurso (que es efectivamente 'agregado'
 juntos para formar todo el proceso general) pueden ser completamente independientes
 y diferente, por lo que es muy importante recordar que el uso de esta identificación
 siempre debe ser puramente opcional (ya que los IRI mismos siempre deben ser
 considerado como completamente opaco, y nunca debe codificar significativo
 semántica en las 'partes' de sus IRI!)."""@es .

#
# Authentication.
#
inrupt_common:UserCredentialResource a rdfs:Class ;
    rdfs:isDefinedBy inrupt_common: ;
    rdfs:label "Class of User Credential Resources"@en ;
    rdfs:label "Clase de recursos de credenciales de usuario"@es ;
    rdfs:comment """A user credential resource contains credentials needed to access various
 APIs, which can include APIs provided by 3rd-parties."""@en ;
    rdfs:comment """Un recurso de credenciales de usuario contiene las credenciales necesarias para
 acceder a varias API, que pueden incluir API proporcionadas por terceros."""@es .

inrupt_common:AuthenticationResponse a rdfs:Class ;
    rdfs:isDefinedBy inrupt_common: ;
    rdfs:label "Class of Authentication Responses"@en ;
    rdfs:label "Clase de respuestas de autenticación"@es ;
    rdfs:comment """Type used to denote a response from an authentication request (expected to
 contain things like access tokens, user IDs, account IDs, etc., when authenticating with an API)."""@en ;
    rdfs:comment """Tipo utilizado para denotar una respuesta de una solicitud de autenticación (se
 espera que contenga elementos como tokens de acceso, ID de usuario, ID de cuenta, etc., al
 autenticarse con una API)."""@es .


inrupt_common:authenticationTokenAsJwt a rdf:Property ;
    rdfs:isDefinedBy inrupt_common: ;
    rdfs:label "Authentication token as JWT"@en ;
    rdfs:label "Token de autenticación como JWT"@es ;
    rdfs:comment """An authentication token encoded as a JSON Web Token (JWT). This JWT may
 contain not just an access code, but also user account IDs or other information."""@en ;
    rdfs:comment """Un token de autenticación codificado como JSON Web Token (JWT). Este JWT puede
 contener no solo un código de acceso, sino también ID de cuenta de usuario u otra información."""@es .

inrupt_common:accessTokenAsString a rdf:Property ;
    rdfs:isDefinedBy inrupt_common: ;
    rdfs:label "Access token (as string)"@en ;
    rdfs:label "Token de acceso (como cadena)"@es ;
    rdfs:comment """An access token, typically used to access an API, represented as a simple string value."""@en ;
    rdfs:comment """Un token de acceso, normalmente utilizado para acceder a una API, representado
 como un valor de cadena simple."""@es .

#
# Working with external data sources.
#
inrupt_common:DataSourceContainer a rdfs:Class ;
    rdfs:isDefinedBy inrupt_common: ;
    rdfs:label "Class of data source containers"@en ;
    rdfs:label "Clase de contenedores de fuentes de datos"@es ;
    rdfs:comment "The class of containers for all data from a particular data source."@en ;
    rdfs:comment "La clase de contenedores para todos los datos de una fuente de datos en particular."@es .

inrupt_common:dataSourceContainer a rdf:Property, owl:ObjectProperty ;
    rdfs:isDefinedBy inrupt_common: ;
    rdfs:label "Data source container"@en ;
    rdfs:label "Contenedor de fuente de datos"@es ;
    rdfs:comment "Container for all data from a particular data source."@en ;
    rdfs:comment "Contenedor para todos los datos de una fuente de datos en particular."@es .

#
# Terms used across generic ETL processes.
#
inrupt_common:etlPushCredentialResourceToPod a rdf:Property, owl:ObjectProperty ;
    rdfs:isDefinedBy inrupt_common: ;
    rdfs:label "ETL - push credential resource to Pod"@en ;
    rdfs:label "ETL: enviar el recurso de credenciales al Pod"@es ;
    rdfs:comment "Flag to tell our customer ETL process to push local customer credentials to their Pod."@en ;
    rdfs:comment "Marcar para indicarle al proceso ETL de nuestro cliente que envíe las credenciales del cliente local a su Pod."@es .

inrupt_common:webId a rdf:Property, owl:ObjectProperty ;
    rdfs:isDefinedBy inrupt_common: ;
    rdfs:seeAlso <https://dvcs.w3.org/hg/WebID/raw-file/tip/spec/identity-respec.html> ;
    rdfs:label "WebID"@en ;
    rdfs:label "WebID"@es ;
    rdfs:comment "A WebID is an identifier, typically for the owner of a Solid Pod (e.g., could be an individual, or a company, or an application, etc.)."@en ;
    rdfs:comment "Un WebID es un identificador, generalmente para el propietario de un Solid Pod (por ejemplo, podría ser un individuo, una empresa, una aplicación, etc.)."@es .


inrupt_common:storageRoot a rdf:Property, owl:ObjectProperty ;
    rdfs:isDefinedBy inrupt_common: ;
    rdfs:seeAlso <https://solidproject.org/TR/protocol#storage> ;
    rdfs:label "Storage root"@en ;
    rdfs:label "Raíz de almacenamiento"@es ;
    rdfs:comment "The IRI of the root resource of a Solid Pod."@en ;
    rdfs:comment "El IRI del recurso raíz de un Solid Pod."@es .

inrupt_common:CredentialResource a rdfs:Class, owl:Class ;
     rdfs:isDefinedBy inrupt_common: ;
     rdfs:label "Class of Credential Resources"@en ;
     rdfs:label "Clase de recursos de credenciales"@es ;
     rdfs:comment """A credential resource contains credentials needed to access various APIs or services, which can include APIs provided by 3rd-parties, or credentials to act as a registered application, etc."""@en ;
     rdfs:comment """Un recurso de credenciales contiene las credenciales necesarias para acceder a varias API o servicios, que pueden incluir API proporcionadas por terceros o credenciales para actuar como una aplicación registrada, etc."""@es .

inrupt_common:clientId a rdf:Property, owl:ObjectProperty ;
    rdfs:isDefinedBy inrupt_common: ;
    rdfs:seeAlso <https://datatracker.ietf.org/doc/html/rfc6749#section-2.2> ;
    rdfs:label "Client ID"@en ;
    rdfs:label "Client ID"@es ;
    rdfs:comment "The OIDC client identifier value, used by registered client applications to identify themselves to an identity provider."@en ;
    rdfs:comment "El valor del identificador de cliente de OIDC, utilizado por las aplicaciones de cliente registradas para identificarse ante un proveedor de identidad."@es .

inrupt_common:clientSecret a rdf:Property, owl:ObjectProperty ;
    rdfs:isDefinedBy inrupt_common: ;
    rdfs:seeAlso <https://datatracker.ietf.org/doc/html/rfc6749#section-2.2> ;
    rdfs:label "Client secret"@en ;
    rdfs:label "Secreta del cliente"@es ;
    rdfs:comment "The OIDC client secret value, used by registered client applications to authenticate themselves to an identity provider."@en ;
    rdfs:comment "El valor secreto del cliente OIDC, utilizado por las aplicaciones cliente registradas para autenticarse ante un proveedor de identidad."@es .

inrupt_common:triplestoreEndpointUpdate a rdf:Property, owl:ObjectProperty ;
    rdfs:isDefinedBy inrupt_common: ;
    rdfs:label "Triplestore endpoint update"@en ;
    rdfs:label "Actualización del punto final de Triplestore"@es ;
    rdfs:comment "This should be a string representation of the endpoint URL for triplestore update requests."@en ;
    rdfs:comment "Debe ser una representación de cadena de la URL del punto final para las solicitudes de actualización de triplestore."@es .

inrupt_common:triplestoreNamedGraph a rdf:Property, owl:ObjectProperty ;
    rdfs:isDefinedBy inrupt_common: ;
    rdfs:label "Triplestore Named Graph"@en ;
    rdfs:label "Gráfico con nombre de Triplestore"@es ;
    rdfs:comment "Named graph to use to represent an individual Solid Pod (e.g., multiple users can have their Pods within their own Named Graph in a single triplestore database instance)."@en ;
    rdfs:comment "Gráfico con nombre que se utiliza para representar un Solid Pod individual (p. Ej., Varios usuarios pueden tener sus Pods dentro de su propio Gráfico con nombre en una única instancia de base de datos de triple almacén)."@es .


inrupt_common:NotificationContainer a rdf:Class, owl:Class ;
    rdfs:isDefinedBy inrupt_common: ;
    rdfs:label "Notification container"@en ;
    rdfs:label "Contenedor de notificaciones"@es ;
    rdfs:comment "The class of notification containers."@en ;
    rdfs:comment "La clase de contenedores de notificación."@es .


inrupt_common:eventSource a rdf:Property, owl:ObjectProperty ;
    rdfs:isDefinedBy inrupt_common: ;
    rdfs:label "Event source"@en ;
    rdfs:label "Origen del evento"@es ;
    rdfs:comment "The source of an event, represented as an IRI identifying that source (e.g., some 3rd party API)."@en ;
    rdfs:comment "La fuente de un evento, representada como un IRI que identifica esa fuente (por ejemplo, alguna API de terceros)."@es .


inrupt_common:eventType a rdf:Property, owl:ObjectProperty ;
    rdfs:isDefinedBy inrupt_common: ;
    rdfs:label "Event type"@en ;
    rdfs:label "Tipo de evento"@es ;
    rdfs:comment "The specific type of event (e.g., a water leak detected, or an appliance turning on or off, etc.)."@en ;
    rdfs:comment "El tipo específico de evento (por ejemplo, una fuga de agua detectada o un aparato que se enciende o apaga, etc.)."@es .

inrupt_common:archived a rdf:Property, owl:ObjectProperty ;
    rdfs:isDefinedBy inrupt_common: ;
    rdfs:label "Archived"@en ;
    rdfs:label "Archivado"@es ;
    rdfs:comment "Whether the subject has been marked as archived, without being deleted."@en ;
    rdfs:comment "Si el asunto se ha marcado como archivado, sin eliminarlo."@es .

#
# Unstable, as I prefer demonstrating reuse of DPV-PD via its very specific
# terms to denote categories and instances of data (mostly from a personal
# data perspective, which seems to fit the general application of Solid, but
# of course isn't 'just' for personal data!).
#
inrupt_common:Tag a rdfs:Class, owl:Class ;
    rdfs:isDefinedBy inrupt_common: ;
    vs:term_status "unstable" ;
    owl:deprecated "true"^^xsd:boolean ;
    rdfs:seeAlso <https://w3id.org/dpv/dpv-pd#> ;
    rdfs:label "Tag"@en ;
    rdfs:label "Etiqueta"@es ;
    rdfs:comment "The class of tags - i.e., to associate an entity with a simple 'Tag', for example using Personal Data Categories from the DPV PD vocab."@en ;
    rdfs:comment "La clase de etiquetas, es decir, para asociar una entidad con una 'Etiqueta' simple, por ejemplo, utilizando Categorías de datos personales del vocabulario DPV PD."@es .

#
# Unstable, as I prefer demonstrating reuse of Gist via its term:
#   gist:isCategorizedBy
#
inrupt_common:tag a rdf:Property, owl:ObjectProperty ;
    rdfs:isDefinedBy inrupt_common: ;
    vs:term_status "unstable" ;
    owl:deprecated "true"^^xsd:boolean ;
    rdfs:label "Tag"@en ;
    rdfs:label "Etiqueta"@es ;
    rdfs:comment "Property used to denote that an entity has a specific tag."@en ;
    rdfs:comment "Propiedad utilizada para indicar que una entidad tiene una etiqueta específica."@es .

#
#inrupt_common: a rdf:Property, owl:ObjectProperty ;
#    rdfs:isDefinedBy inrupt_common: ;
#    rdfs:label ""@en ;
#    rdfs:label ""@es ;
#    rdfs:comment ""@en ;
#    rdfs:comment ""@es .
